src/ORSet.thy
@@ -97,7 +97,7 @@ using assms by(auto simp add: apply_operations_def intro: hb.convergence_ext con
 
 context orset begin
 
-sublocale crdt: op_based_crdt weak_hb hb interpret_op
+sublocale sec: strong_eventual_consistency weak_hb hb interpret_op
   "\<lambda>ops.\<exists>xs i. xs prefix of i \<and> node_deliver_messages xs = ops" "Map.empty"
   apply standard
   apply(erule exE)+
